Progress

MonadicHHL/HHLMonads.lean
@@ -17,11 +17,37 @@ instance : Monad Set where
   pure := Set.pure
   bind := Set.bind
 
+instance : LawfulMonad Set where
+  pure_bind  :=
+    by
+      intro α β a f
+      simp [Pure.pure, Bind.bind, Set.pure, Set.bind]
+  bind_pure_comp  :=
+    by
+      intro α ma
+      simp [Pure.pure, Bind.bind, Set.pure, Set.bind]
+      sorry
+  bind_assoc :=
+    by
+      intro α β γ f g ma
+      simp [Bind.bind, Set.bind]
+      apply Set.ext
+      aesop
+  seqLeft_eq := sorry
+  seqRight_eq := sorry
+  pure_seq := sorry
+  bind_map := sorry
+
 lemma prove_prop_by_eq {α : Type} {x y : α}
   (P : α → Prop)
   (h : x = y) :
   P x ↔ P y := by
     rw [h]
+
+def optionify {α β : Type} {m : Type → Type} [Monad m]
+  (f : α → m (Option β)) : Option α → m (Option β)
+  | some a => f a
+  | none   => pure none
 
 --------------------------------
 -------- HHL typeclass ---------
@@ -88,16 +114,30 @@ lemma WP_bind {α₁ α₂ α₃ : Type}
     aesop
 
 ------------------------------------------------
--------- Transformers Instantiations -----------
+---------------- Base Monads -------------------
 ------------------------------------------------
 
-#check StateT
+---------------- Id ---------------
+
+instance : HHL Id where
+  elemType := Id
+  relWith f p p' := p' = f p
+  bind_rel := by
+    aesop
+
+---------------- Set ---------------
 
 instance : HHL Set where
   elemType := Id
   relWith C p p' := p' ∈ C p
   bind_rel := by
     aesop
+
+------------------------------------------------
+-------- Transformers Instantiations -----------
+------------------------------------------------
+
+------------ StateT ---------------
 
 instance (σ : Type) (m : Type → Type) [Monad m] [HHL m] : HHL (StateT σ m) where
   elemType α := elemType m (α × σ)
@@ -110,7 +150,6 @@ instance (σ : Type) (m : Type → Type) [Monad m] [HHL m] : HHL (StateT σ m) w
     rename_i x0 HHL_M x2 HHL_m
     apply HHL_m.bind_rel (fun v₁ ↦ C₁ v₁.1 v₁.2) (fun v₂ ↦ C₂ v₂.1 v₂.2) p₀ p₂
 
--- Correct StateT σ Set instance
 
 variable (σ : Type)
 -- #check (HHL.relWith (M := StateT σ Set))
@@ -125,23 +164,7 @@ lemma test_stateT_set2 {σ α : Type}
   : relWith C p p' ↔ p' ∈ C p.1 p.2 := by
   rfl
 
--- variable (σ : Type)
--- #check (HHL.relWith (M := StateT σ Set))
--- #synth HHL (StateT σ Set)
-
-/-
-def optionify {α β : Type} {m : Type → Type} [Monad m]
-  (f : α → m (Option β)) : α → m β :=
-  fun a => do
-    match (← f a) with
-    | some b => pure b
-    | none   => fail
--/
-
-def optionify {α β : Type} {m : Type → Type} [Monad m]
-  (f : α → m (Option β)) : Option α → m (Option β)
-  | some a => f a
-  | none   => pure none
+------------ OptionT ---------------
 
 instance (m : Type → Type) [Monad m] [HHL m] [LawfulMonad m] : HHL (OptionT m) where
   elemType α := elemType m (Option α)
@@ -179,14 +202,6 @@ instance (m : Type → Type) [Monad m] [HHL m] [LawfulMonad m] : HHL (OptionT m)
       }
     aesop
 
-instance : HHL Id where
-  elemType := Id
-  relWith f p p' := p' = f p
-  bind_rel := by
-    aesop
-
-
--- Correct HHL Option instance
 
 -- #check (HHL.relWith (M := StateT σ Set))
 -- set_option diagnostics true
@@ -206,433 +221,128 @@ lemma test_HHL_Option2 {α : Type}
     simp [HHL.relWith, optionify, pure]
     aesop
 
+------------ Logical Variables ---------------
 
+--- The unused type parameter is the logical part of the state
+def LogicT (_ : Type) (m : Type _ → Type _) : Type _ → Type _
+ := m
 
+instance (L : Type) (m : Type _ → Type _) [M : Monad m] : Monad (LogicT L m) where
+  pure := M.pure
+  bind := M.bind
 
+/-
+def logicify {L : Type} {m : Type _ → Type _} [Monad m]
+  (f : α → LogicT L m β) (x : α × L) : m β × L :=
+    (f x.1, x.2)
+-/
 
-
-
-instance : HHL Option where
-  elemType α := Option α
-  relWith f p p' :=
-    match p with
-    | none => p' = none
-    | some v => p' = some (f v)
+-- Like StateT basically?
+-- How does this compose with the set base monad?
+instance {m : Type _ → Type _} (L : Type) [Monad m] [HHL m] : HHL (LogicT L m) where
+  elemType α := elemType m α × L
+  --elemType α := elemType m (α × L)
+  relWith --C p p' :=
+   {α β : Type} (C : α → LogicT L m β)
+   --(p : elemType m (α × L)) (p' : elemType m (β × L)) :=
+   (p : elemType m α × L) (p' : elemType m β × L) :=
+    @relWith m _ _ _ _ C p.1 p'.1
+    ∧ p.2 = p'.2
+    --relWith (logicify C) p p'
+    -- relWith (fun v ↦ C v v) p p'
   bind_rel := by
-    simp [Bind.bind, Option.bind]
     intro α₀ α₁ α₂ C₁ C₂ p₀ p₂
-    cases p₀
-    · simp
-    simp
-    cases p₂
-    {
-      simp
-      intro x h1 h2
-      cases x
-      · simp at h1
-      simp at h2
-    }
-    {
-      simp
-      rename_i v0 v2
-      apply Iff.intro
-      {
-        intro h
-        simp at h
-        cases hC₁ : C₁ v0 <;> simp [hC₁] at h
-        rename_i v1
-        apply Exists.intro (some v1)
-        aesop
-      }
-      {
-        intro h
-        simp at h
-        rcases h with ⟨p1, hrel1, hrel2⟩
-        cases hp1 : p1 <;> simp [hp1] at hrel1 hrel2
-        rename_i v1
-        aesop
-      }
-    }
-
-------------------------------------------------
-------------- Instantiations -------------------
-------------------------------------------------
-
-
-
-instance (σ : Type) : HHL (StateM σ) where
-  elemType α := α × σ
-  relWith C p p' := p' = C p.1 p.2
-  bind_rel := by
+    rename_i Monad_M HHL_M Monad_m HHL_m
+    have h := HHL_m.bind_rel C₁ C₂ p₀.1 p₂.1
     aesop
 
-def Set.pure {α : Type} : α → Set α
-  | a => {a}
+abbrev LHHL_Monad (L σ α : Type) : Type :=
+  LogicT L (StateT σ Set) α
 
-def Set.bind {α β : Type} : Set α → (α → Set β) → Set β
-  | S, f => {b | ∃a, a ∈ S ∧ b ∈ f a}
+lemma rel_with_LHHL_Monad (L σ α : Type)
+  (C : α → LHHL_Monad L σ α)
+  (p : (α × σ) × L) (p' : (α × σ) × L) :
+  HHL.relWith C p p' ↔ (p.2 = p'.2 ∧ p'.1 ∈ C p.1.1 p.1.2)
+  := by
+  simp [HHL.relWith]
+  aesop
 
-instance : Monad Set where
-  pure := Set.pure
-  bind := Set.bind
-instance (σ : Type) : HHL (StateT σ Set) where
-  elemType α := α × σ
-  relWith C p p' := p' ∈ C p.1 p.2
-  bind_rel := by
-    simp [Bind.bind, StateT.bind, Set.bind]
+abbrev weird_monad (L σ α : Type) : Type :=
+  StateT σ (LogicT L Set) α
 
-instance : HHL Option where
-  elemType α := Option α
-  relWith f p p' :=
-    match p with
-    | none => p' = none
-    | some v => p' = some (f v)
-  bind_rel := by
-    simp [Bind.bind, Option.bind]
-    intro α₀ α₁ α₂ C₁ C₂ p₀ p₂
-    cases p₀
-    · simp
-    simp
-    cases p₂
-    {
-      simp
-      intro x h1 h2
-      cases x
-      · simp at h1
-      simp at h2
-    }
-    {
-      simp
-      rename_i v0 v2
-      apply Iff.intro
-      {
-        intro h
-        simp at h
-        cases hC₁ : C₁ v0 <;> simp [hC₁] at h
-        rename_i v1
-        apply Exists.intro (some v1)
-        aesop
-      }
-      {
-        intro h
-        simp at h
-        rcases h with ⟨p1, hrel1, hrel2⟩
-        cases hp1 : p1 <;> simp [hp1] at hrel1 hrel2
-        rename_i v1
-        aesop
-      }
-    }
+lemma both_commute_ (L σ α : Type) :
+  (HHL.elemType (weird_monad L σ) α) = (HHL.elemType (LHHL_Monad L σ) α) :=
+  rfl
+
+lemma both_commute_rel_with (L σ α : Type) :
+  (HHL.elemType (weird_monad L σ) α) = (HHL.elemType (LHHL_Monad L σ) α) :=
+  rfl
+
+
+
+-- The two monad transformers commute???
+
+
+
+lemma rel_with_weird (L σ α : Type)
+  (C : α → weird_monad L σ α)
+  (p : (α × σ) × L) (p' : (α × σ) × L) :
+  HHL.relWith C p p' ↔ (p.2 = p'.2) -- ∧ p'.1 ∈ C p.1.1 p.1.2)
+  := by
+  simp [HHL.relWith]
+  sorry
+  --aesop
+
+
 
 
 end HHL
 
-namespace StateNonDetAlt
 
--- Parameters
+abbrev HHL_Monad (σ α : Type) : Type :=
+  StateT σ Set α
 
--- Computational monad:
-def M (σ α : Type) : Type :=
-  σ → Set (α × σ)
+lemma semify_for_HHL {σ α₁ α₂ : Type}
+  (C : α₁ → HHL_Monad σ α₂) (S : Set (α₁ × σ)) :
+  HHL.semify C S = { p' | ∃ p ∈ S, p' ∈ C p.1 p.2 }
+:= rfl
 
-def pure {σ α : Type} (x : α) : M σ α :=
-  fun σ => {(x, σ)}
+abbrev Hypra_Monad (σ α : Type) : Type :=
+  OptionT (StateT σ Set) α
 
-def bind {σ α₁ α₂ : Type}
-  (C₁ : M σ α₁) (C₂ : α₁ → M σ α₂) : M σ α₂ :=
-  fun σ => (⋃p' ∈ C₁ σ, C₂ p'.1 p'.2)
+variable {σ : Type}
+#synth HHL (StateT σ Set)
+#synth LawfulMonad (OptionT (StateT σ Set))
+#synth HHL (OptionT (StateT σ Set))
 
-instance (σ : Type) : Monad (M σ) where
-  pure := pure
-  bind := bind
-
--- Abstraction in the logic
-def ElemType (σ α : Type) : Type :=
-  α × σ
-
-def rel_with {σ α₁ α₂ : Type}
-  (C : α₁ → M σ α₂) (p : ElemType σ α₁) (p' : ElemType σ α₂)
-   : Prop :=
-  p' ∈ C p.1 p.2
-
--- Sequential composition
-
-lemma interaction_bind_rel {σ α₁ α₂ : Type}
-  (C₁ : α₀ → M σ α₁)
-  (C₂ : α₁ → M σ α₂)
-  (p₀ : ElemType σ α₀)
-  (p₂ : ElemType σ α₂) :
-  rel_with (fun v₁ ↦ bind (C₁ v₁) C₂) p₀ p₂
-↔ ∃ p₁, rel_with C₁ p₀ p₁ ∧ rel_with C₂ p₁ p₂
+lemma relWith_Hypra {σ α₁ α₂ : Type}
+  (C : α₁ → Hypra_Monad σ α₂)
+  (p : Option α₁ × σ)
+  (p' : Option α₂ × σ) :
+  HHL.relWith C p p' ↔
+    (p.1 = none ∧ p'.1 = none ∧ p.2 = p'.2) ∨
+    (∃ v, p.1 = some v ∧ p' ∈ C v p.2)
 := by
-  simp [rel_with, bind]
-  aesop
-
--------------------------
--------- Generic --------
--------------------------
-
-def semify {σ α₁ α₂ : Type}
-  (C : α₁ → M σ α₂) : Set (ElemType σ α₁) → Set (ElemType σ α₂) :=
-  fun S => { p' | ∃ p ∈ S, rel_with C p p'}
-
-
-lemma semify_bind {σ α₁ α₂ α₃ : Type}
-  (C₁ : α₁ → M σ α₂)
-  (C₂ : α₂ → M σ α₃)
-  (S : Set (ElemType σ α₁))
-  :
- semify (fun v₁ ↦ bind (C₁ v₁) C₂) S = semify C₂ (semify C₁ S)
- := by
-  simp [semify]
-  apply Set.ext
-  intro p'
-  simp
-  have h := interaction_bind_rel C₁ C₂
-  aesop
-
-def hyperassertion (σ α : Type) : Type :=
-  Set (ElemType σ α) → Prop
-
-def W (σ α₁ α₂ : Type) : Type :=
-  hyperassertion σ α₂ → hyperassertion σ α₁
-
-def WP {σ α₁ α₂ : Type}
-  (C : α₁ → M σ α₂) : W σ α₁ α₂ :=
-  fun Q S => Q (semify C S)
-
-lemma WP_bind {σ α₁ α₂ α₃ : Type}
-  (C₁ : α₁ → M σ α₂)
-  (C₂ : α₂ → M σ α₃) :
-  WP (fun v₁ => C₁ v₁ >>= C₂) = (WP C₁) ∘ (WP C₂)
-  := by
-    apply funext
-    intro Q
-    apply funext
-    intro S
-    apply propext
-    simp [WP, Bind.bind]
-    apply prove_prop_by_eq
-    have h := semify_bind C₁ C₂ S
-    aesop
-
-end StateNonDetAlt
-
-
-
-
-universe u v w
-
-section SetBaseMonad
-
-/-
-def SetT (m : Type u -> Type v) (α : Type u) : Type _ :=
-  Set (m α)
-
-def SetT (m : Type u -> Type v) (α : Type u) : Type _ :=
-  m (Set α)
--/
-
-
-
-instance Set.LawfulMonad : LawfulMonad Set :=
+  simp [HHL.relWith, optionify, pure]
+  cases p.1
   {
-    pure_bind  :=
-      by
-        intro α β a f
-        simp [Pure.pure, Bind.bind, Set.pure, Set.bind]
-    bind_pure_comp  :=
-      by
-        intro α ma
-        simp [Pure.pure, Bind.bind, Set.pure, Set.bind]
-        sorry
-    bind_assoc :=
-      by
-        intro α β γ f g ma
-        simp [Bind.bind, Set.bind]
-        apply Set.ext
-        aesop
-    seqLeft_eq := sorry
-    seqRight_eq := sorry
-    pure_seq := sorry
-    bind_map := sorry }
+    simp
+    simp [StateT.pure, pure, Set.pure]
+    grind
+  }
+  simp
 
-
-def set_bind_state {α val : Type} (S : Set (val × α)) (C : (val × α) → Set (val × α)) : Set (val × α) :=
-  { y | ∃ x ∈ S, y ∈ C x }
-
-abbrev HHL_monad (α : Type) : Type → Type :=
-  StateT α Set
-
-lemma HHL_monad_simpler (α val : Type) :
-  HHL_monad α val = (α → Set (val × α)) := by
-    simp [HHL_monad, StateT]
-
-lemma HHL_monad_same_bind {α : Type} (C₁ : HHL_monad α Unit) (C₂ : Unit → HHL_monad α Unit) :
-  C₁ >>= C₂ = (fun σ => set_bind_state (C₁ σ) (fun (_, σ') => C₂ () σ'))
-  := by
-    aesop
-
-lemma HHL_monad_same_bind_val {α val : Type}
-  (C₁ : HHL_monad α val) (C₂ : val → HHL_monad α val) :
-  C₁ >>= C₂ = (fun σ => set_bind_state (C₁ σ) (fun (x, σ') => C₂ x σ'))
-  := by
-    aesop
-
--- with option for errors
-
-abbrev Hypra_monad (α : Type) : Type → Type :=
-  OptionT (StateT α Set)
-
-lemma Hypra_monad_simpler (α val : Type) :
-  Hypra_monad α val = (α → Set (Option val × α)) := by
-    simp [Hypra_monad, OptionT, StateT]
-
-
-def set_bind_state_hypra {α val : Type}
-  (S : Set (Option val × α))
-  (C : (val × α) → Set (Option val × α)) : Set (Option val × α) :=
-  { y | ∃ x ∈ S,
-  (
-    match x with
-    | (none, σ) => y = (none, σ)
-    | (some v, σ) => y ∈ C (v, σ)
-  )}
-
-
-
-lemma Hypra_monad_same_bind {α : Type} (C₁ : Hypra_monad α Unit) (C₂ : Unit → Hypra_monad α Unit) :
-  C₁ >>= C₂ = (fun σ => set_bind_state_hypra (C₁ σ) (fun (_, σ') => C₂ () σ'))
-  := by
-    simp [Hypra_monad, set_bind_state_hypra, bind, OptionT.bind, OptionT.mk]
-    apply funext
-    intro x
-    refine Set.ext ?_
-    intro y
-    simp [StateT.bind]
-    apply Iff.intro
-    {
-      intro yin
-      rcases yin with ⟨a, ha, hcase⟩
-      apply Exists.intro a.fst
-      apply Exists.intro a.snd
-      apply And.intro
-      assumption
-      simp
-      cases a with
-      | mk o σ =>
-        cases o with
-        | none =>
-            simpa using hcase
-        | some v =>
-            cases v
-            simpa using hcase
-    }
-    {
-      intro h
-      rcases h with ⟨a, ha, ⟨hcase, hh⟩⟩
-      simp [bind, Set.bind]
-      apply Exists.intro a
-      apply Exists.intro ha
-      apply And.intro hcase
-      cases a
-      simp [pure, StateT.pure, Set.pure]
-      aesop
-      simp
-      aesop
-    }
-
-lemma Hypra_monad_same_bind_val {α val : Type}
-  (C₁ : Hypra_monad α val) (C₂ : val → Hypra_monad α val) :
-  C₁ >>= C₂ = (fun σ => set_bind_state_hypra (C₁ σ) (fun (x, σ') => C₂ x σ'))
-  := by
-    simp [Hypra_monad, set_bind_state_hypra, bind, OptionT.bind, OptionT.mk]
-    apply funext
-    intro x
-    refine Set.ext ?_
-    intro y
-    simp [StateT.bind]
-    apply Iff.intro
-    {
-      intro yin
-      rcases yin with ⟨a, ha, hcase⟩
-      apply Exists.intro a.fst
-      apply Exists.intro a.snd
-      apply And.intro
-      assumption
-      simp
-      cases a with
-      | mk o σ =>
-        cases o with
-        | none =>
-            simpa using hcase
-        | some v =>
-            simpa using hcase
-    }
-    {
-      intro h
-      rcases h with ⟨a, ha, ⟨hcase, hh⟩⟩
-      simp [bind, Set.bind]
-      apply Exists.intro a
-      apply Exists.intro ha
-      apply And.intro hcase
-      cases a
-      simp [pure, StateT.pure, Set.pure]
-      aesop
-      simp
-      aesop
-    }
-
-abbrev Var : Type :=
-  String
-
-def SState (α : Type) : Type :=
-  Var → α
-
-abbrev HypraM (α val : Type) : Type :=
-  -- State α → Set (Option α × State α)
-  OptionT (StateT (SState α) Set) val
-
-lemma simpler_HypraM (α val : Type) :
-  HypraM α val = (SState α → Set (Option val × SState α)) := by
-    simp [HypraM, OptionT, StateT]
-
-abbrev HHLMonad (α val : Type) : Type :=
-  -- State α → Set (Option α × State α)
-  StateT (SState α) Set val
-
-
-lemma simpler_HHLMonad (α val : Type _) :
-  HHLMonad α val = (SState α → Set (val × SState α)) := by
-    simp [HHLMonad, StateT]
-
-example (α L : Type _) :
-  (HHLMonad α L → L) = ((SState α → Set (L × SState α)) → L)
-  := by simp [HHLMonad, StateT]
-
-
-example (α : Type) :
-  (HypraM α (Prop × Prop) → (Prop × Prop))
-  =
-  ((SState α → Set (Option (Prop × Prop) × SState α)) → Prop × Prop)
+lemma semify_for_Hypra {σ α₁ α₂ : Type}
+  (C : α₁ → Hypra_Monad σ α₂) (S : Set (Option α₁ × σ)) :
+  HHL.semify C S =
+  { p' | ∃ p ∈ S, (p.1 = none ∧ p'.1 = none ∧ p.2 = p'.2) ∨ (∃ v, p.1 = some v ∧ p' ∈ C v p.2) }
 := by
-  simp [HypraM, OptionT, StateT]
-
-
-/-
-instance : MAlgOrdered (StateM Int) (Int → Prop) where
-  μ (f : Int → (Int → Prop) × Int) :=
-    fun b =>
-      let (post, b') := f b
-      post b'
-  μ_ord_pure := sorry
-  μ_ord_bind := sorry
--/
-
-example (α : Type) :
-  HHLMonad α (Set (SState α) → Prop) = (SState α → Set ((Set (SState α) → Prop) × SState α)) := by
-    simp [HHLMonad, StateT]
-
-#check StateT
+  simp [HHL.semify]
+  have h := relWith_Hypra C
+  apply Set.ext
+  intro x
+  simp
+  sorry
 
 
 syntax (name := checkUnfolding) "#check " term " unfolding " ident* : command
@@ -655,563 +365,6 @@ def elacCheckUnfolding : CommandElab
   | _ => throwUnsupportedSyntax
 
 
-abbrev MonadT : Type _ :=
-  (Type _ → Type _) → Type _ → Type _
+abbrev MonadT : Type _ := (Type _ → Type _) → Type _ → Type _
 
-
-
-
--- Do we even need the set in the computation monad?
--- How to get non-det?
--- Do I just get a monad then?
---def HyperM (T : MonadT) (α : Type _) : Type _ :=
---  T Set α
---  T Set α
-
--- Computation monad:
--- OptionT (StateT (SState α) Set)
--- OptionT (StateT σ) Set)
--- with α = σ → Set (Option α × σ)
-
-namespace Id
-
------ Step 1
------ Id
-def M (α : Type) : Type :=
-  α
-
-def pure {α : Type} (x : α) : Id.M α :=
-  x
-
-def bind {α β : Type}
-  (ma : Id.M α)
-  (f : α → Id.M β) : Id.M β :=
-  f ma
-
-instance : Monad Id.M where
-  pure := Id.pure
-  bind := Id.bind
-
-def hyperassertion (α : Type) : Type :=
-  Set α → Prop
-
-def W (α₁ α₂ : Type) : Type :=
-  Id.hyperassertion α₂ → Id.hyperassertion α₁
-
-def WP {α₁ α₂ : Type}
-  (C : α₁ → Id.M α₂) : Id.W α₁ α₂ :=
-  fun Q S => Q (C '' S)
-
-lemma WP_bind {α₁ α₂ α₃ : Type}
-  (C₁ : α₁ → Id.M α₂)
-  (C₂ : α₂ → Id.M α₃) :
-  Id.WP (fun v₁ => C₁ v₁ >>= C₂) = (Id.WP C₁) ∘ (Id.WP C₂)
-  := by
-    apply funext
-    intro Q
-    apply funext
-    intro S
-    apply propext
-    simp [Id.WP, Set.image, Bind.bind, Id.bind]
-
-end Id
-
-----------------------------------------
------- Adding set
-----------------------------------------
-
-namespace NonDet
-
-def M (α : Type) : Type :=
-  Set α
-
-instance : Monad M where
-  pure := Set.pure
-  bind := Set.bind
-
-def hyperassertion (α : Type) : Type :=
-  Set α → Prop
-
-def W (α₁ α₂ : Type) : Type :=
-  hyperassertion α₂ → hyperassertion α₁
-
-def WP {α₁ α₂ : Type}
-  (C : α₁ → M α₂) : W α₁ α₂ :=
-  fun Q S => Q (⋃σ∈S, C σ)
-
-lemma WP_bind {α₁ α₂ α₃ : Type}
-  (C₁ : α₁ → M α₂)
-  (C₂ : α₂ → M α₃) :
-  WP (fun v₁ => C₁ v₁ >>= C₂) = (WP C₁) ∘ (WP C₂)
-  := by
-    apply funext
-    intro Q
-    apply funext
-    intro S
-    apply propext
-    simp [WP, Bind.bind, Set.bind]
-    apply prove_prop_by_eq
-    apply Set.ext
-    intro p'
-    simp
-    aesop
-
-end NonDet
-
-namespace State
-
-def M (σ α : Type) : Type :=
-  σ → α × σ
-
-def pure {σ α : Type} (x : α) : M σ α :=
-  fun s => (x, s)
-
-def bind {σ α₁ α₂ : Type}
-  (ma : M σ α₁)
-  (f : α₁ → M σ α₂) : M σ α₂ :=
-  fun s =>
-    let (a, s') := ma s
-    f a s'
-
-instance (σ : Type) : Monad (M σ) where
-  pure := pure
-  bind := bind
-
-def hyperassertion (σ α : Type) : Type :=
-  Set (α × σ) → Prop
-
-def W (σ α₁ α₂ : Type) : Type :=
-  hyperassertion σ α₂ → hyperassertion σ α₁
-
-def WP {σ α₁ α₂ : Type}
-  (C : α₁ → M σ α₂) : W σ α₁ α₂ :=
-  fun Q S => Q { p' | ∃ v σ, (v, σ) ∈ S ∧ p' = C v σ }
-
-lemma WP_bind {σ α₁ α₂ α₃ : Type}
-  (C₁ : α₁ → M σ α₂)
-  (C₂ : α₂ → M σ α₃) :
-  WP (fun v₁ => C₁ v₁ >>= C₂) = (WP C₁) ∘ (WP C₂)
-  := by
-    apply funext
-    intro Q
-    apply funext
-    intro S
-    apply propext
-    simp [WP, Bind.bind, bind]
-    grind
-
-
-end State
-
-namespace StateNonDet
-
--- Parameters
-
-def M (σ α : Type) : Type :=
-  σ → Set (α × σ)
-
-def pure {σ α : Type} (x : α) : M σ α :=
-  fun σ => {(x, σ)}
-
-def bind {σ α₁ α₂ : Type}
-  (C₁ : M σ α₁) (C₂ : α₁ → M σ α₂) : M σ α₂ :=
-  fun σ => (⋃p' ∈ C₁ σ, C₂ p'.1 p'.2)
-
-instance (σ : Type) : Monad (M σ) where
-  pure := pure
-  bind := bind
-
-def ElemType (σ α : Type) : Type :=
-  α × σ
-
-def semify {σ α₁ α₂ : Type}
-  (C : α₁ → M σ α₂) : Set (ElemType σ α₁) → Set (ElemType σ α₂) :=
-    fun S => (⋃p∈S, C p.1 p.2)
-
-lemma semify_bind {σ α₁ α₂ α₃ : Type}
-  (C₁ : α₁ → M σ α₂)
-  (C₂ : α₂ → M σ α₃)
-  (S : Set (ElemType σ α₁))
-  :
- semify (fun v₁ ↦ bind (C₁ v₁) C₂) S = semify C₂ (semify C₁ S)
- := by
-  simp [semify, bind]
-  aesop
-
-------------------------------
--- Generic
-------------------------------
-
-def hyperassertion (σ α : Type) : Type :=
-  Set (ElemType σ α) → Prop
-
-def W (σ α₁ α₂ : Type) : Type :=
-  hyperassertion σ α₂ → hyperassertion σ α₁
-
-def WP {σ α₁ α₂ : Type}
-  (C : α₁ → M σ α₂) : W σ α₁ α₂ :=
-  fun Q S => Q (semify C S)
-
-lemma WP_bind {σ α₁ α₂ α₃ : Type}
-  (C₁ : α₁ → M σ α₂)
-  (C₂ : α₂ → M σ α₃) :
-  WP (fun v₁ => C₁ v₁ >>= C₂) = (WP C₁) ∘ (WP C₂)
-  := by
-    apply funext
-    intro Q
-    apply funext
-    intro S
-    apply propext
-    simp [WP, Bind.bind]
-    apply prove_prop_by_eq
-    have h := semify_bind C₁ C₂ S
-    aesop
-
-end StateNonDet
-
-
-semify (fun v₁ ↦ bind (C₁ v₁) C₂) S = semify C₂ (semify C₁ S)
-
-
--------------------- Older stuff
-
-
-
-def HyperM (σ : Type) : Type → Type :=
-  OptionT (StateT σ Set)
-
-example (α σ : Type) :
-  HyperM σ α = (σ → Set (Option α × σ)) := by
-    simp [HyperM, OptionT, StateT]
-
-
--- What's the morphism?
-
----- Instantiations
-
--- T = Id
--- HyperM T α = α
--- HyperW T α = (Set α → Prop) → (Set α → Prop)
-
--- HyperM is just the monad?
-
--- T = State σ
--- HyperM T α = σ → α × σ
--- HyperW T α₁ α₂ = (Set (α₂ × σ) → Prop) → (Set (α₂ × σ) → Prop)
-
-
--- T = ?
--- HyperM T α = σ → Set (α × σ)
--- HyperW T α₁ α₂ = (Set (α₂ × σ) → Prop) → (Set (α₂ × σ) → Prop)
-
--- T = ?
--- HyperM T α = Set α
--- HyperW T α₁ α₂ = (Set α₂ → Prop) → (Set α₁ → Prop)
-
--- ...
--- Computation monad := σ → Set (Option α × σ)
--- HyperW α₁ α₂ = (Set (Option α₂ × σ) → Prop) → (Set (Option α₁ × σ) → Prop)
-
-
-
-
-
-
-example (α val : Type) :
-  (HyperM (StateT α) val) = (α → Set (val × α)) := by
-  simp [HyperM, StateT]
-
-def HyperW (T : MonadT) (α : Type) : Type :=
-  (Set (val₂ × α) → Prop) → Set (val₁ × α) → Prop
-
-def HyperW (α val₁ val₂ : Type) : Type :=
-  (Set (val₂ × α) → Prop) → Set (val₁ × α) → Prop
-  -- post → pre
-
-
-
-abbrev HyperM (α val : Type) : Type :=
-  -- α → Set (val × α)
-  StateT α Set val
-
-example (α val : Type) :
-  HyperM α val = (α → Set (val × α)) := by
-    simp [HyperM, StateT]
-
-def hyperassertion (α : Type) : Type :=
-  Set α → Prop
-
-def HyperW (α val₁ val₂ : Type) : Type :=
-  (Set (val₂ × α) → Prop) → Set (val₁ × α) → Prop
-  -- post → pre
-
-def WP {α val₁ val₂ : Type}
-  (C : val₁ → HyperM α val₂) : HyperW α val₁ val₂ :=
-  fun post S =>
-    post { p' | ∃ v σ, (v, σ) ∈ S ∧ p' ∈ C v σ }
-
-def bind_like_WP {α val₁ val₂ val₃ : Type}
-  (WP1 : HyperW α val₁ val₂) (WP2 : HyperW α val₂ val₃)
-  : HyperW α val₁ val₃ :=
-  WP1 ∘ WP2
-
-#check WP
-#print WP
-#reduce WP
-#reduce (types := true) WP
-
-#check WP
-#check WP unfolding HyperW HyperM StateT
-
--- syntax (name := elabCheckDsimp) "#check_dsimp " term : command
-
-
-
-
-
-lemma WP_bind_works {α val₁ val₂ val₃ : Type}
-  (C₁ : val₁ → HyperM α val₂)
-  (C₂ : val₂ → HyperM α val₃) :
-  WP (fun v₁ => C₁ v₁ >>= C₂) = bind_like_WP (WP C₁) (WP C₂)
-  := by
-    apply funext
-    intro Q
-    apply funext
-    intro S
-    apply propext
-    simp  [bind_like_WP, bind, WP, StateT.bind, Set.bind]
-    apply prove_prop_by_eq
-    apply Set.ext
-    intro p'
-    aesop
-
-
-#check WP
-#check WP unfolding HyperW HyperM StateT
-
-def WP_pure {α val₁ val₂ : Type} (x : val₂) : HyperW α val₁ val₂ :=
-  fun (post : Set (val₂ × α) → Prop) (S : Set (val₁ × α)) =>
-    post {  p | ∃ v σ, (v, σ) ∈ S ∧ p = (x, σ) }
-
-def pureM {α val : Type} (x : val) : HyperM α val :=
-  fun σ => {(x, σ)}
-
--- Kinda useless?
-lemma WP_pure_works {α val₁ val₂ : Type}
-  (x : val₂) :
-  WP (fun (_ : val₁) => pureM x)
-  = (WP_pure x: HyperW α val₁ val₂)
-  := by
-    apply funext
-    intro Q
-    apply funext
-    intro S
-    simp [WP, pureM, WP_pure]
-
-/-
-nection is given by the morphism WPStateM : StateM σ α → StateW σ α defined as follows:  WPStateM (m : StateM σ α) ≜ λ post (s : σ). let (res, s′) = (m s) in post res s′ (3)
--/
-def WP {α val : Type}
-  (C : HyperM α val) : HyperW α val :=
-  fun post S =>
-    post { (v, σ') | ∃ σ ∈ S, (v, σ') ∈ C σ }
-
--- we add the return to every state in S
-def WP.pure {α val : Type} (x : val) : HyperW α val :=
-  fun (post : Set (val × α) → Prop) (S : Set α) =>
-    post { (x, σ) | σ ∈ S }
-
-def StateW.bind {α val₁ val₂ : Type}
-  (w : HyperW α val₁)
-  (f : val₁ → HyperW α val₂) : HyperW α val₂ :=
-  fun
-    (post : Set (val₂ × α) → Prop)
-    (S : Set α)
-    =>
-    w
-      (fun (S' : Set (val₁ × α)) => ∀ (v₁ : val₁) (σ' : α),
-        (v₁, σ') ∈ S' →
-        f v₁ post {σ' })
-      S
-
--- What does bind mean in this context???
--- Specification monad doesn't work with relational reasoning?
-def WP.bind {α val₁ val₂ : Type}
-  (w : HyperW α val₁)
-  (f : val₁ → HyperW α val₂) : HyperW α val₂ :=
-  fun
-    (post : Set (val₂ × α) → Prop)
-    (S : Set α)
-    =>
-    sorry
-
--- WP(C1; C2, Q) = WP(C1, WP(C2, Q))
-
-def WP.bind_unit {α val₂ : Type}
-  (WP1 : HyperW α Unit)
-  (WP2 : Unit → HyperW α val₂) : HyperW α val₂ :=
-  --WP1 : Set (Unit × α) → Prop) → (Set α → Prop)
-  fun (Q : Set (val₂ × α) → Prop) (S : Set α) =>
-    have RR : Set α → Prop := WP2 () Q
-    have R : Set (Unit × α) → Prop :=
-      fun S' => RR (Prod.snd '' S')
-    WP1 R S
-
-/-
-  (Set (val × α) → Prop) → (Set α → Prop)
-      (fun (S' : Set (Unit × α)) => ∀ (σ' : α),
-        ((), σ') ∈ S' →
-        f () post {σ' })
-      S
-  -/
-
-
-
-/-
-∀x, WP (pureM x) = pureW x (4)  ∀m f , WP (bindM m f ) = bindW (WP m) (λr . WP (f r )) (5)
--/
-
-instance (α : Type) : MAlgOrdered (HyperM α) (Set α → Prop) where
-  μ (f : α → Set ((Set α → Prop) × α)) :=
-    fun S: Set α =>
-      -- let SS : Set (Set ((Set α → Prop) × α)) := f '' S
-      let SS : Set ((Set α → Prop) × α) := (⋃σ∈S, f σ)
-      -- Intuitively: I have a set of initial states S, and I create the set of reachable states from all initial states
-      -- What do I do with all my postconditions?
-      let posts : Set (Set α → Prop) := Prod.fst '' SS
-      let S' : Set α := Prod.snd '' SS
-      -- need non-emptiness for mu_ord_pure
-      ∀ post ∈ posts, post S'
-  μ_ord_pure := by
-    simp [pure, StateT.pure, Set.pure, Set.image]
-    intro P
-    apply funext
-    intro S
-    -- if exists: ⊢ ((∃ x, x ∈ S) ∧ P S) = P S
-    -- if forall: ⊢ (∀ post,  ∀ x ∈ S, post = P → post S) = P S
-
-    refine propext ?_
-    apply Iff.intro
-    {
-      -- cannot prove existence of postcondition
-      -- aesop
-      sorry
-    }
-    {
-      -- needs non-emptiness for this case
-      /-
-      intro h
-      rcases h with ⟨post, postIn, hpost⟩
-      specialize hpost P
-      exact hpost
-      -/
-      sorry
-    }
-
-  μ_ord_bind := by
-    simp [Bind.bind, Set.image, StateT.bind, Set.bind, Pi.hasLe]
-    intro α f g x1 x2 x3 x4 x5
-    intro x6 x7 x8 x9 x10 x11 x12
-
-
-
-    sorry
-
-
-instance (α : Type) : MAlgOrdered (HHLMonadAbstract α) (Set α → Prop) where
-  μ (f : α → Set ((Set α → Prop) × α)) :=
-    fun S: Set α =>
-      -- let SS : Set (Set ((Set α → Prop) × α)) := f '' S
-      let SS : Set ((Set α → Prop) × α) := (⋃σ∈S, f σ)
-      -- Intuitively: I have a set of initial states S, and I create the set of reachable states from all initial states
-      -- What do I do with all my postconditions?
-      let posts : Set (Set α → Prop) := Prod.fst '' SS
-      let S' : Set α := Prod.snd '' SS
-      -- need non-emptiness for mu_ord_pure
-      (∃σ, σ ∈ S') ∧ (∀ post ∈ posts, post S')
-  μ_ord_pure := by
-    simp [pure, StateT.pure, Set.pure, Set.image]
-    intro P
-    apply funext
-    intro S
-    refine propext ?_
-    apply Iff.intro
-    {
-      -- needs non-emptiness for this case
-      aesop
-      /-
-      intro h
-      rcases h with ⟨hex, h⟩
-      rcases hex with ⟨x, xS⟩
-      specialize h P x
-      -/
-    }
-    {
-      -- cannot prove existence of x
-      aesop
-      sorry
-    }
-
-
-
-  μ_ord_bind := by
-    simp [Bind.bind, Set.bind]
-    intro α f g
-    sorry
-
--- μ : HHLMonad α (Set (State α) → Prop) → Set (State α) → Prop
-instance : MAlgOrdered Set Prop where
--- instance (α : Type) : MAlgOrdered (HHLMonad α) Prop where
-  μ := (fun S => (∀ x ∈ S, x) ∧ (∃x ∈ S, x))
-  μ_ord_pure := by
-    simp [pure, Set.pure]
-    aesop
-  μ_ord_bind := by
-    simp [Bind.bind, Set.bind]
-    intro α f g h1 S h2
-    intro P x hxS hPfx hP
-    simp [Pi.hasLe] at h1
-    apply And.intro
-    {
-      intro Q y hyS Qgy
-      apply h2
-      exact hxS
-      -- could also use x
-
-      specialize h1 y
-
-
-
-
-      sorry
-    }
-    {
-
-      sorry
-    }
-
-
-
-
-instance (α : Type) : MAlgOrdered (HypraM α) (Set (State α) → Prop) where
-  μ := (fun S => (∀ x ∈ S, x) ∧ (∃x ∈ S, x))
-  μ_ord_pure := by
-    simp [pure, Set.pure]
-    aesop
-  μ_ord_bind := by
-    simp [Bind.bind, Set.bind]
-    intro α f g
-    sorry
-
-instance : MAlgOrdered Set Prop where
-  μ := (fun S => (∀ x ∈ S, x) ∧ (∃x ∈ S, x))
-  μ_ord_pure := by
-    simp [pure, Set.pure]
-    aesop
-  μ_ord_bind := by
-    simp [Bind.bind, Set.bind]
-    intro α f g
-    sorry
-
-instance (σ : Type u) : MAlgOrdered (Set σ) (Set σ → Prop) where
-instance (σ : Type u) : MAlgOrdered (σ → Prop) ((σ → Prop) → Prop) where
+end
